repeat ourselves

stdpp/base.v
@@ -758,7 +758,9 @@ Lemma uncurry4_curry4 {A B C D E} (f : A * B * C * D → E) p :
 Proof. destruct p as [[[??] ?] ?]; reflexivity. Qed.
 
 (** [pair_eq] as a name is more consistent with our usual naming. *)
-Definition pair_eq {A B} := @pair_equal_spec A B.
+Lemma pair_eq {A B} (a1 a2 : A) (b1 b2 : B) :
+  (a1, b1) = (a2, b2) ↔ a1 = a2 ∧ b1 = b2.
+Proof. apply pair_equal_spec. Qed.
 Global Instance pair_inj {A B} : Inj2 (=) (=) (=) (@pair A B).
 Proof. injection 1; auto. Qed.
 Global Instance prod_map_inj {A A' B B'} (f : A → A') (g : B → B') :
